Update Core.lean

src/Init/Core.lean
@@ -2310,6 +2310,13 @@ instance Pi.instSubsingleton {α : Sort u} {β : α → Sort v} [∀ a, Subsingl
 
 /-! # Squash -/
 
+theorem equivalence_true (α : Sort u) : Equivalence fun _ _ : α ↦ True :=
+  ⟨fun _ ↦ trivial, fun _ ↦ trivial, fun _ _ ↦ trivial⟩
+
+/-- Always-true relation as a `Setoid`. -/
+protected def Setoid.trivial (α : Sort u) : Setoid α :=
+  ⟨_, equivalence_true α⟩
+
 /--
 The quotient of `α` by the universal relation. The elements of `Squash α` are those of `α`, but all
 of them are equal and cannot be distinguished.
@@ -2323,8 +2330,12 @@ and its representation in compiled code is identical to that of `α`.
 
 Consequently, `Squash.lift` may extract an `α` value into any subsingleton type `β`, while
 `Nonempty.rec` can only do the same when `β` is a proposition.
+
+We define `Squash` in terms of `Quotient` rather than just `Quot`. This means that
+`Squash` can be used when a `Quotient` argument is expected, and the setoid will be
+automatically inferred.
 -/
-def Squash (α : Sort u) := Quot (fun (_ _ : α) => True)
+def Squash (α : Sort u) := Quotient (Setoid.trivial α)
 
 /--
 Places a value into its squash type, in which it cannot be distinguished from any other.
